pulse/ulib/LowStar.RST.fsti
@@ -21,15 +21,19 @@ module HST = FStar.HyperStack.ST
 module A = LowStar.Array
 module R = LowStar.Resource
 
-/// The `RST` effect is the top concept of the Steel framework. It offers a way of specifying function in terms of resources, abstracting
-/// away the `modifies` theory of `LowStar.Array`.
+/// The `RST` effect is the top concept of the Steel framework. It offers a way of specifying
+/// function in terms of resources, abstracting away the `modifies` theory of `LowStar.Array`.
 
-(**** Abstract modifies clause for the resource-indexed state effect *)
+(****
+  Abstract modifies clause for the resource-indexed
+  state effect
+*)
 
-/// Because this new state effect will only talk about heap modifications structured in terms of resources, we can refine the notion of
-/// `modifies`. More precisely, if `l1` is modified into `l2` when going from heap `h0` to heap `h1`, then every other used region of
-/// the heap stays disjoint from the modifies region and stays used. It morally means that any growth in the modified region induced by
-/// a function does not touch existing used locations.
+/// Because this new state effect will only talk about heap modifications structured in terms of
+/// resources, we can refine the notion of `modifies`. More precisely, if `l1` is modified into `l2`
+/// when going from heap `h0` to heap `h1`, then every other used region of the heap stays disjoint
+/// from the modifies region and stays used. It morally means that any growth in the modified region
+/// induced by a function does not touch existing used locations.
 let frame_usedness_preservation (l1 l2:A.loc) (h0 h1:HS.mem) = forall (frame: A.loc).
  (A.loc_disjoint frame l1 /\ A.loc_includes (A.loc_used_in h0) frame) ==>
    (A.loc_disjoint frame l2 /\ A.loc_includes (A.loc_used_in h1) frame)
@@ -43,7 +47,10 @@ val frame_usedness_preservation_intro (l1 l2: A.loc) (h0 h1:HS.mem)
 
 val frame_usedness_preservation_elim (l1 l2: A.loc) (h0 h1:HS.mem) (frame: A.loc)
   : Lemma
-    (requires (frame_usedness_preservation l1 l2 h0 h1 /\ (A.loc_disjoint frame l1) /\ A.loc_includes (A.loc_used_in h0) frame))
+    (requires (
+      frame_usedness_preservation l1 l2 h0 h1 /\ (A.loc_disjoint frame l1) /\
+      A.loc_includes (A.loc_used_in h0) frame)
+    )
     (ensures (A.loc_disjoint frame l2 /\ A.loc_includes (A.loc_used_in h1) frame))
 
 /// We can now define our new `modifies` in terms of resources.
@@ -68,7 +75,8 @@ val modifies_trans (res0 res1 res2:R.resource) (h0 h1 h2:HS.mem)
 
 (**** Subresources *)
 
-/// `LowStar.Resource` defines `can_be_split_into`, but we need here an existential predicate to not carry around all the splitting deltas.
+/// `LowStar.Resource` defines `can_be_split_into`, but we need here an existential predicate to not
+/// carry around all the splitting deltas.
 val is_subresource_of (r0 r: R.resource) : Type0
 
 val is_subresource_of_elim
@@ -101,61 +109,69 @@ val is_subresource_of_trans (r1 r2 r3: R.resource)
   : Lemma
     (requires (r1 `is_subresource_of` r2 /\ r2 `is_subresource_of` r3))
     (ensures (r1 `is_subresource_of` r3))
-  [SMTPat (r1 `is_subresource_of` r2); SMTPat (r2 `is_subresource_of` r3); SMTPat (r1 `is_subresource_of` r3)]
+  [SMTPat (r1 `is_subresource_of` r2); SMTPat (r2 `is_subresource_of` r3);
+   SMTPat (r1 `is_subresource_of` r3)]
 
-val is_subresource_of_refl (r: R.resource) : Lemma(r `is_subresource_of` r) [SMTPat (r `is_subresource_of` r)]
+val is_subresource_of_refl (r: R.resource) : Lemma(r `is_subresource_of` r)
+  [SMTPat (r `is_subresource_of` r)]
 
 (**** Selectors *)
 
-/// The spirit of `LowStar.Resource` is to limit our reasonning to a fragment of the heap. For the `RST` effect, we push this idea
-/// further and we will no longer allow to speak about the entirety of the heap inside pre and postconditions. Rather, we want to be only
-/// able to talk about the resources at hand.
+/// The spirit of `LowStar.Resource` is to limit our reasonning to a fragment of the heap. For the
+/// `RST` effect, we push this idea further and we will no longer allow to speak about the entirety
+/// of the heap inside pre and postconditions. Rather, we want to be only able to talk about the
+/// resources at hand.
 
 module Fext =  FStar.FunctionalExtensionality
 
-/// We extend on the `LowStar.Resource.sel_t` selector type by allowing our new selectors to also talk about the subresources contained
-/// inside the enclosing resource. Selectors are morally `(r0:R.resource{r0 is_subresource_of r}) -> r0.R.t`, but we need to define
-/// them with functional extensionality.
-let selector (r: R.resource) : Type = Fext.restricted_g_t (r0:R.resource{r0 `is_subresource_of` r}) (fun r0 -> r0.R.t)
+/// We extend on the `LowStar.Resource.sel_t` selector type by allowing our new selectors to also
+/// talk about the subresources contained inside the enclosing resource. Selectors are morally
+/// `(r0:R.resource{r0 is_subresource_of r}) -> r0.R.t`, but we need to define them with functional
+/// extensionality. Since selectors are morally a heap restricted to a resource, we call them rmem.
+let rmem (r: R.resource) : Type =
+  Fext.restricted_g_t (r0:R.resource{r0 `is_subresource_of` r}) (fun r0 -> r0.R.t)
 
-/// The main way to make a selector is to derive one from a particular state of the heap. `mk_selector r h` effectively restricts your
-/// access to the heap to accesses that are valid and withing the resource you consider.
-val mk_selector
+/// The main way to make a selector is to derive one from a particular state of the heap.
+/// `mk_rmem r h` effectively restricts your access to the heap to accesses that are valid and
+/// within the resource you consider.
+val mk_rmem
   (r: R.resource)
   (h: R.imem (R.inv r)) :
-  Tot (s:selector r{forall (r0:R.resource{r0 `is_subresource_of` r}). s r0 == R.sel r0.R.view h})
+  Tot (rh:rmem r{forall (r0:R.resource{r0 `is_subresource_of` r}). rh r0 == R.sel r0.R.view h})
 
 /// The only other transformation allowed on selectors is focusing on a subresource.
-val focus_selector (#r: R.resource) (s: selector r) (r0: R.resource{r0 `is_subresource_of` r})
-  : Tot (selector r0)
+val focus_rmem (#r: R.resource) (h: rmem r) (r0: R.resource{r0 `is_subresource_of` r})
+  : Tot (rmem r0)
 
-val focus_selector_equality (outer inner: R.resource) (h: HS.mem)
+val focus_rmem_equality (outer inner: R.resource) (h: HS.mem)
   : Lemma
     (requires (R.inv outer h /\ inner `is_subresource_of` outer))
     (ensures (is_subresource_of_elim inner outer (R.inv inner h) (fun _ -> ());
-      focus_selector (mk_selector outer h) inner == mk_selector inner h))
+      focus_rmem (mk_rmem outer h) inner == mk_rmem inner h))
     [SMTPatOr [
-      [SMTPat (focus_selector (mk_selector outer h) inner)];
-      [SMTPat (mk_selector inner h); SMTPat (inner `is_subresource_of` outer)]
+      [SMTPat (focus_rmem (mk_rmem outer h) inner)];
+      [SMTPat (mk_rmem inner h); SMTPat (inner `is_subresource_of` outer)]
     ]]
 
-/// In the ST state, pre and postconditions depended on the entire heap. Here, theses conditions depend only on a `selector` for the
-/// resource at hand (derived from a heap state).
-let sprop r = selector r -> Type0
+/// In the ST state, pre and postconditions depended on the entire heap. Here, theses conditions
+/// depend only on a `rmem` for the resource at hand (derived from a heap state).
+let rprop r = rmem r -> Type0
 
-/// `extend_sprop` is the dual of `focus_selector`.
-val extend_sprop (#r0: R.resource) (p: sprop r0) (r: R.resource{r0 `is_subresource_of` r}) : Tot (sprop r)
+/// `extend_rprop` is the dual of `focus_rmem`.
+val extend_rprop (#r0: R.resource) (p: rprop r0) (r: R.resource{r0 `is_subresource_of` r})
+  : Tot (rprop r)
 
-// /// Thanks to selectors, we can define abstract resource refinements that strenghten the invariant of a resource.
-val hsrefine (r:R.resource) (p:sprop r) : Tot (r':R.resource{
+/// Thanks to selectors, we can define abstract resource refinements that strenghten the invariant
+/// of a resource.
+val hsrefine (r:R.resource) (p:rprop r) : Tot (r':R.resource{
     r'.R.t == r.R.t /\
-    r'.R.view == {r.R.view with R.inv = fun h -> r.R.view.R.inv h /\ p (mk_selector r h)}
+    r'.R.view == {r.R.view with R.inv = fun h -> r.R.view.R.inv h /\ p (mk_rmem r h)}
   })
 
 (**** The RST effect *)
 
-/// On top of the invariants of the resource at hand, we add another global invariant governing how resources are used :
-/// The footprint of resources used in Steel functions have to be used.
+/// On top of the invariants of the resource at hand, we add another global invariant governing how
+/// resources are used : the footprint of resources used in Steel functions have to be used.
 val rst_inv (res:R.resource) (h:HS.mem) : GTot prop
 
 val reveal_rst_inv (_ : unit)
@@ -168,48 +184,55 @@ val rst_inv_star (res0 res1: R.resource) (h: HS.mem)
   : Lemma (rst_inv R.(res0 <*> res1) h <==> rst_inv R.(res1 <*> res0) h)
   [SMTPat (rst_inv R.(res0 <*> res1) h)]
 
-let r_pre (res:R.resource) =  sprop res
+let r_pre (res:R.resource) =  rprop res
 let r_post
   (res0: R.resource)
   (a: Type)
   (res1: a -> R.resource) =
-  selector res0 -> x:a -> sprop (res1 x)
+  rmem res0 -> x:a -> rprop (res1 x)
 
 
-/// Finally, the RST effect. Eventually with the layered effects, its definition will be hidden here. It has five indexes:
+/// Finally, the RST effect. Eventually with the layered effects, its definition will be hidden
+/// here. It has five indexes:
 ///  * the return type;
-///  * the initial resource, which is the composite heap object formed by all the arguments to the function;
-///  * the final resource, which is the composite heap object alive at then end of the function (and depends on the return value);
-///  * the precondition, which is an `sprop` of the initial resource and should be used to indicate the functional specification of the
-///    function, since all of the memory shape specification has been dealt with in the two previous indexes;
-///  * the postcondition, function of the initial and final resources selectors and the return value.
-/// The pre/postcondition of the `ST` effect have been split in two. First, you specify what happens to the memory: what heap objects are
-/// live at the beginning, how the function transforms this memory shape. Then, you can add traditionnal functional specification but,
-/// thanks to selectors, these functional specification can only depend on the views of the resources you're handling.
+///  * the initial resource, which is the composite heap object formed by all the arguments to the
+///    function;
+///  * the final resource, which is the composite heap object alive at then end of the function
+///    (and depends on the return value);
+///  * the precondition, which is an `rprop` of the initial resource and should be used to indicate
+///    the functional specification of the function, since all of the memory shape specification has
+///    been dealt with in the two previous indexes;
+///  * the postcondition, function of the initial and final resources selectors and the return
+///    value.
+/// The pre/postcondition of the `ST` effect have been split in two. First, you specify what happens
+/// to the memory: what heap objects are live at the beginning, how the function transforms this
+/// memory shape. Then, you can add traditionnal functional specification but, thanks to selectors,
+/// these functional specification can only depend on the views of the resources you're handling.
 effect RST
   (a: Type)
   (res0: R.resource)
   (res1: a -> R.resource)
-  (pre: sprop res0)
-  (post: selector res0 -> (x:a) -> sprop (res1 x))
+  (pre: rprop res0)
+  (post: rmem res0 -> (x:a) -> rprop (res1 x))
 = ST.ST
   a
-  (fun h0 -> R.inv res0 h0 /\ rst_inv res0 h0 /\ pre (mk_selector res0 h0))
+  (fun h0 -> R.inv res0 h0 /\ rst_inv res0 h0 /\ pre (mk_rmem res0 h0))
   (fun h0 x h1 ->
-    R.inv res0 h0 /\ rst_inv res0 h0 /\ pre (mk_selector res0 h0) /\
+    R.inv res0 h0 /\ rst_inv res0 h0 /\ pre (mk_rmem res0 h0) /\
     R.inv (res1 x) h1 /\
     rst_inv (res1 x) h1 /\
     modifies res0 (res1 x) h0 h1 /\
-    post (mk_selector res0 h0) x (mk_selector (res1 x) h1)
+    post (mk_rmem res0 h0) x (mk_rmem (res1 x) h1)
   )
 
-/// Similar to `FStar.Hyperstack.ST.get`, this helper gives you a selector based on the current state of the heap
+/// Similar to `FStar.Hyperstack.ST.get`, this helper gives you a rmem based on the current state of
+/// the heap
 val get (r: R.resource) : RST
-  (selector r)
+  (rmem r)
   (r)
   (fun _ -> r)
   (fun _ -> True)
-  (fun old returned cur -> returned == old /\ old == cur)
+  (fun h0 h h1 -> h == h0 /\ h0 == h1)
 
 
 (**** The frame rule *)
@@ -218,15 +241,20 @@ val get (r: R.resource) : RST
 
 open LowStar.RST.Tactics
 
-/// Finally, the workhorse separation logic rule that will be pervasive in Steel programs: the frame rule. All calls to RST functions
-/// should be encapsulated inside `rst_frame`. The rule takes 3 mandatory arguments:
-///  * `outer0` is the resource summming up all the live heap objects when the function `f` is called;
-///  * `outer1 x` is the resource summing up all the live heap objects after the function `f` returns with return value `x`;
-///  * `f` is the RST function you want to call, with pre and post resources `inner0` and `outer1 x`.
-/// Morally, you want to call `f` on `inner0` which is a fraction of your `outer0` resource context. What this rule does is to find
-/// automatically (thanks to a tactic) the `delta` such that `outer0 == inner0 <*> delta`. Then it checks that the `outer1 x` you
-/// provided does indeed satisfy `outer1 x == inner1 x <*> delta`. The postcondition of `f` is propagated to `outer1`, as well as the
-/// core information provided by the frame rule: the `delta` does not change.
+/// Finally, the workhorse separation logic rule that will be pervasive in Steel programs: the frame
+/// rule. All calls to RST functions should be encapsulated inside `rst_frame`. The rule takes 3
+/// mandatory arguments:
+///  * `outer0` is the resource summming up all the live heap objects when the function `f` is
+///    called;
+///  * `outer1 x` is the resource summing up all the live heap objects after the function `f`
+///    returns with return value `x`;
+///  * `f` is the RST function you want to call, with pre and post resources `inner0` and
+///    `outer1 x`.
+/// Morally, you want to call `f` on `inner0` which is a fraction of your `outer0` resource context.
+/// What this rule does is to find automatically (thanks to a tactic) the `delta` such that
+/// `outer0 == inner0 <*> delta`. Then it checks that the `outer1 x` you provided does indeed
+/// satisfy `outer1 x == inner1 x <*> delta`. The postcondition of `f` is propagated to `outer1`,
+/// as well as the core information provided by the frame rule: the `delta` does not change.
 inline_for_extraction noextract val rst_frame
   (outer0:R.resource)
   (#inner0:R.resource)
@@ -240,20 +268,21 @@ inline_for_extraction noextract val rst_frame
          (frame_delta outer0 inner0 outer1 inner1 delta)
      }
    )
-  (#pre:sprop inner0)
-  (#post:selector inner0 -> (x:a) -> sprop (inner1 x))
+  (#pre:rprop inner0)
+  (#post:rmem inner0 -> (x:a) -> rprop (inner1 x))
    ($f:unit -> RST a inner0 inner1 pre post)
   : RST a outer0 outer1
-    (FStar.Tactics.by_tactic_seman resolve_frame_delta (frame_delta outer0 inner0 outer1 inner1 delta);
-      fun old ->
-        pre (focus_selector old inner0)
+    (FStar.Tactics.by_tactic_seman resolve_frame_delta
+      (frame_delta outer0 inner0 outer1 inner1 delta);
+      fun h ->
+        pre (focus_rmem h inner0)
     )
     (R.reveal_can_be_split_into ();
-      fun old x cur ->
+      fun h0 x h1 ->
         post
-          (focus_selector old inner0)
+          (focus_rmem h0 inner0)
           x
-          (focus_selector cur (inner1 x)) /\
+          (focus_rmem h1 (inner1 x)) /\
         (assert(delta `is_subresource_of` outer0); assert(delta `is_subresource_of` outer1 x);
-        focus_selector old delta == focus_selector cur delta)
+        focus_rmem h0 delta == focus_rmem h1 delta)
     )
