pulse/ulib/LowStar.RST.Loops.fsti
@@ -11,42 +11,42 @@ open FStar.Mul
 inline_for_extraction
 val while
   (res:resource)
-  (inv: (selector res -> Type0))
-  (guard: (selector res -> GTot bool))
+  (inv: (rmem res -> Type0))
+  (guard: (rmem res -> GTot bool))
   (test: (unit -> RST bool
     res
     (fun _ -> res)
-    (requires fun old -> inv old)
-    (ensures fun old b cur ->
-      b == guard old /\
-      old == cur)
+    (requires fun h -> inv h)
+    (ensures fun h0 b h1 ->
+      b == guard h0 /\
+      h0 == h1)
   ))
   (body: (unit -> RST unit
     res
     (fun _ -> res)
-    (requires fun old -> guard old /\ inv old)
-    (ensures fun old _ cur -> inv cur)
+    (requires fun h -> guard h /\ inv h)
+    (ensures fun h0 _ h1 -> inv h1)
   ))
   : RST unit
     res
     (fun _ -> res)
-    (requires fun old -> inv old)
-    (ensures fun _ _ cur -> inv cur /\ ~(guard cur))
+    (requires fun h -> inv h)
+    (ensures fun _ _ h1 -> inv h1 /\ ~(guard h1))
 
 inline_for_extraction
 val for
   (start:U32.t)
   (finish:U32.t{U32.v finish >= U32.v start})
   (context: resource)
-  (loop_inv: (selector context -> nat -> Type0))
+  (loop_inv: (rmem context -> nat -> Type0))
   (f:(i:U32.t{U32.(v start <= v i /\ v i < v finish)} -> RST unit
     (context)
     (fun _ -> context)
-    (requires (fun old -> loop_inv old (U32.v i)))
-    (ensures (fun old _ cur -> U32.(loop_inv old (v i) /\ loop_inv cur (v i + 1))))
+    (requires (fun h -> loop_inv h (U32.v i)))
+    (ensures (fun h0 _ h1 -> U32.(loop_inv h0 (v i) /\ loop_inv h1 (v i + 1))))
   ))
   : RST unit
     (context)
     (fun _ -> context)
-    (requires (fun old -> loop_inv old (U32.v start)))
-    (ensures (fun _ _ cur -> loop_inv cur (U32.v finish)))
+    (requires (fun h -> loop_inv h (U32.v start)))
+    (ensures (fun _ _ h1 -> loop_inv h1 (U32.v finish)))
